proof/old_system/uni/def_extra.v
@@ -1,4 +1,4 @@
-Require Import Metalib.Metatheory.
+Require Export Metalib.Metatheory.
 Require Import List.
 
 Require Import uni.def_ott.
@@ -21,12 +21,40 @@ Fixpoint fvar_in_aworklist' (Γ_5:aworklist) : vars :=
   | (aworklist_conswork Γ w) => (fvar_in_aworklist' Γ) \u (fvar_in_work w)
 end.
   
+Inductive apply_cont : cont -> typ -> work -> Prop :=
+  | apply_cont__infabs: forall A c,
+      apply_cont (cont_infabs c) 
+                   A
+                   (work_infabs A c)
+  | apply_cont__tapp : forall A B c,
+      apply_cont (cont_inftapp B c) 
+                   A
+                   (work_inftapp A B c)
+  | apply_cont__tappunion : forall A2 B C1 c,
+      apply_cont (cont_inftappunion A2 B c) 
+                   C1
+                   (work_inftappunion C1 A2 B c)
+  | apply_cont__unioninftapp : forall A1 A2 c,
+      apply_cont (cont_unioninftapp A1 c) 
+                   A2
+                   (work_unioninftapp A1 A2 c)
+  | apply_cont__sub : forall A B,
+      apply_cont (cont_sub B) 
+                   A
+                   (work_sub A B)
+.
 
-(* Inductive work : Set := 
- | work_infer (e:exp) (c:typ -> work)
- | work_check (e:exp) (A:typ)
- | work_infabs (A:typ) (c:typ -> work)
- | work_infapp (A:typ) (e:exp) (c:typ -> work)
- | work_inftapp (A1:typ) (A2:typ) (c:typ -> work)
- | work_sub (A1:typ) (A2:typ)
- | work_apply (c:typ -> work) (A:typ). *)
+Inductive apply_cont2 : contd -> typ -> typ -> work -> Prop :=
+  | apply_cont2__infapp : forall A B e c,
+      apply_cont2 (contd_infapp e c) 
+                  A B
+                  (work_infapp A B e c)
+  | apply_cont2__infabsunion : forall A2 B1 C1 c, 
+      apply_cont2 (contd_infabsunion A2 c) 
+                  B1 C1
+                  (work_infabsunion B1 C1 A2 c)
+  | apply_cont2__unioninfabs : forall B1 B2 C1 C2 c,
+      apply_cont2 (contd_unioninfabs B1 C1 c) 
+                  B2 C2
+                  (work_unioninfabs B1 C1 B2 C2 c)
+.
